src/Parsers/ContextFreeGrammar/Fix/FromAbstractInterpretationDefinitions.v
@@ -3,7 +3,6 @@ Require Import Coq.Classes.Morphisms.
 Require Import Fiat.Parsers.ContextFreeGrammar.PreNotations.
 Require Import Fiat.Parsers.ContextFreeGrammar.Carriers.
 Require Import Fiat.Parsers.ContextFreeGrammar.Core.
-Require Import Fiat.Parsers.ContextFreeGrammar.Precompute.
 Require Import Fiat.Parsers.BaseTypes.
 Require Import Fiat.Parsers.Splitters.RDPList.
 Require Import Fiat.Parsers.ContextFreeGrammar.Fix.Definitions.
@@ -68,215 +67,193 @@ Section general_fold.
 
   Context (G : pregrammar' Char).
 
-  Global Instance compile_item_data_of_abstract_interpretation : opt.compile_item_data Char state
-    := {| opt.on_terminal := on_terminal;
-          opt.nonterminal_names := pregrammar_nonterminals G;
-          opt.invalid_nonterminal := Gensym.gensym (pregrammar_nonterminals G) |}.
+  Definition fold_item'
+             (fold_nt : default_nonterminal_carrierT -> state)
+             (it : item Char)
+    : state
+    := match it with
+       | Terminal ch => on_terminal ch
+       | NonTerminal nt => fold_nt (@of_nonterminal _ (@rdp_list_predata _ G) nt)
+       end.
 
-  Section with_compiled_productions.
-    Context (compiled_productions : list (opt.productions state)).
+  Global Instance fold_item'_ProperR {R}
+         {R_Reflexive : Reflexive R}
+    : Proper (pointwise_relation _ R ==> eq ==> R) fold_item' | 20.
+  Proof.
+    intros ?? H [?|?] ??; subst; simpl; [ reflexivity | apply H ].
+  Qed.
 
-    Definition opt_Lookup_idx (n : nat) : opt.productions state
-      := List.nth n compiled_productions nil.
-    Lemma eq_opt_Lookup_idx
-          (Hcompiled_productions : List.map opt.compile_productions (List.map snd (pregrammar_productions G)) = compiled_productions)
-          n
-      : opt_Lookup_idx n = opt.compile_productions (Lookup_idx G n).
+  Global Instance fold_item'_Proper
+    : Proper (pointwise_relation _ eq ==> eq ==> eq) fold_item' | 20
+    := _.
+
+  Definition fold_production'
+             (fold_nt : default_nonterminal_carrierT -> state)
+             (its : production Char)
+    := List.fold_right
+         combine_production
+         on_nil_production
+         (List.map
+            (fold_item' fold_nt)
+            its).
+
+  Global Instance fold_production'_ProperR {R}
+         {R_Reflexive : Reflexive R}
+         {combine_production_ProperR : Proper (R ==> R ==> R) combine_production}
+    : Proper (pointwise_relation _ R ==> eq ==> R) fold_production' | 20.
+  Proof.
+    unfold fold_production'.
+    repeat intro.
+    apply (_ : Proper (_ ==> _ ==> SetoidList.eqlistA R ==> _) (@List.fold_right _ _));
+      trivial.
+    subst; apply map_eqlistA_Proper; try reflexivity.
+    repeat intro; apply fold_item'_ProperR; trivial.
+  Qed.
+
+  Global Instance fold_production'_Proper
+    : Proper (pointwise_relation _ eq ==> eq ==> eq) fold_production' | 2
+    := _.
+
+  Global Instance: Params (@fold_production') 5.
+
+  Definition fold_productions'
+             (fold_nt : default_nonterminal_carrierT -> state)
+             (its : productions Char)
+    := List.fold_right
+         least_upper_bound
+         ⊥
+         (List.map
+            (fold_production' fold_nt)
+            its).
+
+  Global Instance fold_productions'_ProperR {R}
+         {R_Reflexive : Reflexive R}
+         {least_upper_bound_ProperR : Proper (R ==> R ==> R) least_upper_bound}
+         {combine_production_ProperR : Proper (R ==> R ==> R) combine_production}
+    : Proper (pointwise_relation _ R ==> eq ==> R) fold_productions' | 20.
+  Proof.
+    unfold fold_production'.
+    repeat intro.
+    apply (_ : Proper (_ ==> _ ==> SetoidList.eqlistA R ==> _) (@List.fold_right _ _));
+      trivial.
+    subst; apply map_eqlistA_Proper; try reflexivity.
+    repeat intro; apply fold_production'_ProperR; trivial.
+  Qed.
+
+  Global Instance fold_productions'_Proper_eq
+    : Proper (pointwise_relation _ eq ==> eq ==> eq) fold_productions' | 20
+    := _.
+
+  Definition fold_constraints
+             (fold_nt : default_nonterminal_carrierT -> state)
+             (nt : default_nonterminal_carrierT)
+    : state
+    := fold_productions'
+         fold_nt
+         (Lookup_idx G nt).
+
+  Section extR.
+    Context (R : state -> state -> Prop)
+            (combine_production_Proper : Proper (R ==> R ==> R) combine_production)
+            (lub_Proper : Proper (R ==> R ==> R) least_upper_bound)
+            (R_Reflexive : Reflexive R).
+
+    Lemma fold_item'_extR {f g} (ext : forall b, R (f b) (g b)) b
+      : R (fold_item' f b) (fold_item' g b).
     Proof.
-      unfold opt_Lookup_idx, Lookup_idx; subst compiled_productions.
-      change nil with (opt.compile_productions nil) at 1.
-      rewrite List.map_nth.
-      reflexivity.
-    Qed.
-
-    Definition fold_item'
-               (fold_nt : default_nonterminal_carrierT -> state)
-               (it : opt.item state)
-      : state
-      := match it with
-         | opt.Terminal tv => tv
-         | opt.NonTerminal nt nt_idx => fold_nt nt_idx
-         end.
-
-    Global Instance fold_item'_ProperR {R}
-           {R_Reflexive : Reflexive R}
-      : Proper (pointwise_relation _ R ==> eq ==> R) fold_item' | 20.
-    Proof.
-      intros ?? H [?|?] ??; subst; simpl; [ reflexivity | apply H ].
-    Qed.
-
-    Global Instance fold_item'_Proper
-      : Proper (pointwise_relation _ eq ==> eq ==> eq) fold_item' | 20
-      := _.
-
-    Definition fold_production'
-               (fold_nt : default_nonterminal_carrierT -> state)
-               (its : opt.production state)
-      := List.fold_right
-           combine_production
-           on_nil_production
-           (List.map
-              (fold_item' fold_nt)
-              its).
-
-    Global Instance fold_production'_ProperR {R}
-           {R_Reflexive : Reflexive R}
-           {combine_production_ProperR : Proper (R ==> R ==> R) combine_production}
-      : Proper (pointwise_relation _ R ==> eq ==> R) fold_production' | 20.
-    Proof.
-      unfold fold_production'.
-      repeat intro.
-      apply (_ : Proper (_ ==> _ ==> SetoidList.eqlistA R ==> _) (@List.fold_right _ _));
-        trivial.
-      subst; apply map_eqlistA_Proper; try reflexivity.
-      repeat intro; apply fold_item'_ProperR; trivial.
-    Qed.
-
-    Global Instance fold_production'_Proper
-      : Proper (pointwise_relation _ eq ==> eq ==> eq) fold_production' | 2
-      := _.
-
-    Global Instance: Params (@fold_production') 5.
-
-    Definition fold_productions'
-               (fold_nt : default_nonterminal_carrierT -> state)
-               (its : opt.productions state)
-      := List.fold_right
-           least_upper_bound
-           ⊥
-           (List.map
-              (fold_production' fold_nt)
-              its).
-
-    Global Instance fold_productions'_ProperR {R}
-           {R_Reflexive : Reflexive R}
-           {least_upper_bound_ProperR : Proper (R ==> R ==> R) least_upper_bound}
-           {combine_production_ProperR : Proper (R ==> R ==> R) combine_production}
-      : Proper (pointwise_relation _ R ==> eq ==> R) fold_productions' | 20.
-    Proof.
-      unfold fold_production'.
-      repeat intro.
-      apply (_ : Proper (_ ==> _ ==> SetoidList.eqlistA R ==> _) (@List.fold_right _ _));
-        trivial.
-      subst; apply map_eqlistA_Proper; try reflexivity.
-      repeat intro; apply fold_production'_ProperR; trivial.
-    Qed.
-
-    Global Instance fold_productions'_Proper_eq
-      : Proper (pointwise_relation _ eq ==> eq ==> eq) fold_productions' | 20
-      := _.
-
-    Definition fold_constraints
-               (fold_nt : default_nonterminal_carrierT -> state)
-               (nt : default_nonterminal_carrierT)
-      : state
-      := fold_productions'
-           fold_nt
-           (opt_Lookup_idx nt).
-
-    Section extR.
-      Context (R : state -> state -> Prop)
-              (combine_production_Proper : Proper (R ==> R ==> R) combine_production)
-              (lub_Proper : Proper (R ==> R ==> R) least_upper_bound)
-              (R_Reflexive : Reflexive R).
-
-      Lemma fold_item'_extR {f g} (ext : forall b, R (f b) (g b)) b
-        : R (fold_item' f b) (fold_item' g b).
-      Proof.
-        unfold fold_item'.
-        generalize (@of_nonterminal _ (@rdp_list_predata _ G)); simpl; intro.
-        generalize on_terminal; intro.
-        unfold state in *.
-        simpl in *.
-        clear -ext R_Reflexive.
-        abstract (destruct b; try apply ext; reflexivity).
-      Defined.
-
-      Lemma fold_production'_extR {f g} (ext : forall b, R (f b) (g b)) b
-        : R (fold_production' f b) (fold_production' g b).
-      Proof.
-        unfold fold_production'.
-        induction b as [ | x ]; try reflexivity; simpl.
-        apply combine_production_Proper; [ apply (fold_item'_extR ext) | apply IHb ].
-      Defined.
-
-      Lemma fold_productions'_extR {f g} (ext : forall b, R (f b) (g b)) b
-        : R (fold_productions' f b) (fold_productions' g b).
-      Proof.
-        unfold fold_productions'.
-        induction b as [ | x ]; try reflexivity; simpl.
-        apply lub_Proper; [ apply (fold_production'_extR ext) | apply IHb ].
-      Defined.
-
-      Lemma fold_constraints_extR f g (H : forall x, R (f x) (g x)) nt
-        : R (fold_constraints f nt) (fold_constraints g nt).
-      Proof.
-        unfold fold_constraints.
-        apply fold_productions'_extR.
-        intro; apply H.
-      Defined.
-    End extR.
-
-    Definition fold_item'_ext {f g} (ext : forall b, f b = g b) b
-      : fold_item' f b = fold_item' g b
-      := fold_item'_extR (R := eq) _ ext b.
-    Definition fold_production'_ext {f g} (ext : forall b, f b = g b) b
-      : fold_production' f b = fold_production' g b
-      := fold_production'_extR (R := eq) _ _ ext b.
-    Definition fold_productions'_ext {f g} (ext : forall b, f b = g b) b
-      : fold_productions' f b = fold_productions' g b
-      := fold_productions'_extR (R := eq) _ _ _ ext b.
-    Definition fold_constraints_ext f g (H : forall x, f x = g x) nt
-      : fold_constraints f nt = fold_constraints g nt
-      := fold_constraints_extR (R := eq) _ _ _ _ _ H nt.
-
-    Definition fold_item'_ext_beq {f g} (ext : forall b, f b =b g b) b
-      : fold_item' f b =b fold_item' g b
-      := fold_item'_extR (R := state_beq) _ ext b.
-    Definition fold_production'_ext_beq
-               {f g} (ext : forall b, f b =b g b) b
-      : fold_production' f b =b fold_production' g b
-      := fold_production'_extR (R := state_beq) _ _ ext b.
-    Definition fold_productions'_ext_beq
-               {f g} (ext : forall b, f b =b g b) b
-      : fold_productions' f b =b fold_productions' g b
-      := fold_productions'_extR (R := state_beq) _ _ _ ext b.
-    Definition fold_constraints_ext_beq
-               f g (H : forall x, f x =b g x) nt
-      : fold_constraints f nt =b fold_constraints g nt
-      := fold_constraints_extR (R := state_beq) _ _ _ _ _ H nt.
-
-    Global Instance fold_constraints_ProperR
-           {R : state -> state -> Prop}
-           {combine_production_Proper : Proper (R ==> R ==> R) combine_production}
-           {lub_Proper : Proper (R ==> R ==> R) least_upper_bound}
-           {R_Reflexive : Reflexive R}
-      : Proper (pointwise_relation default_nonterminal_carrierT R ==> eq ==> R)
-               fold_constraints
-    | 10.
-    Proof.
-      intros f g H; repeat intro; subst.
-      apply fold_constraints_extR; assumption.
+      unfold fold_item'.
+      generalize (@of_nonterminal _ (@rdp_list_predata _ G)); simpl; intro.
+      generalize on_terminal; intro.
+      unfold state in *.
+      simpl in *.
+      clear -ext R_Reflexive.
+      abstract (destruct b; try apply ext; reflexivity).
     Defined.
 
-    Global Instance fold_constraints_Proper
-      : Proper (pointwise_relation default_nonterminal_carrierT eq ==> eq ==> eq)
-               fold_constraints
-      := _.
-
-    Global Instance fold_constraints_Proper_state_beq
-      : Proper (pointwise_relation default_nonterminal_carrierT state_beq ==> eq ==> state_beq)
-               fold_constraints
-      := _.
-
-    Definition fixedpoint_by_abstract_interpretation : grammar_fixedpoint_data.
+    Lemma fold_production'_extR {f g} (ext : forall b, R (f b) (g b)) b
+      : R (fold_production' f b) (fold_production' g b).
     Proof.
-      refine {| prestate := T;
-                step_constraints folder nt st := fold_constraints folder nt;
-                lattice_data := fpdata |}.
-      { repeat intro; apply fold_constraints_Proper_state_beq; assumption. }
+      unfold fold_production'.
+      induction b as [ | x ]; try reflexivity; simpl.
+      apply combine_production_Proper; [ apply (fold_item'_extR ext) | apply IHb ].
     Defined.
-  End with_compiled_productions.
+
+    Lemma fold_productions'_extR {f g} (ext : forall b, R (f b) (g b)) b
+      : R (fold_productions' f b) (fold_productions' g b).
+    Proof.
+      unfold fold_productions'.
+      induction b as [ | x ]; try reflexivity; simpl.
+      apply lub_Proper; [ apply (fold_production'_extR ext) | apply IHb ].
+    Defined.
+
+    Lemma fold_constraints_extR f g (H : forall x, R (f x) (g x)) nt
+      : R (fold_constraints f nt) (fold_constraints g nt).
+    Proof.
+      unfold fold_constraints.
+      apply fold_productions'_extR.
+      intro; apply H.
+    Defined.
+  End extR.
+
+  Definition fold_item'_ext {f g} (ext : forall b, f b = g b) b
+  : fold_item' f b = fold_item' g b
+    := fold_item'_extR (R := eq) _ ext b.
+  Definition fold_production'_ext {f g} (ext : forall b, f b = g b) b
+  : fold_production' f b = fold_production' g b
+    := fold_production'_extR (R := eq) _ _ ext b.
+  Definition fold_productions'_ext {f g} (ext : forall b, f b = g b) b
+  : fold_productions' f b = fold_productions' g b
+    := fold_productions'_extR (R := eq) _ _ _ ext b.
+  Definition fold_constraints_ext f g (H : forall x, f x = g x) nt
+    : fold_constraints f nt = fold_constraints g nt
+    := fold_constraints_extR (R := eq) _ _ _ _ _ H nt.
+
+  Definition fold_item'_ext_beq {f g} (ext : forall b, f b =b g b) b
+  : fold_item' f b =b fold_item' g b
+    := fold_item'_extR (R := state_beq) _ ext b.
+  Definition fold_production'_ext_beq
+             {f g} (ext : forall b, f b =b g b) b
+  : fold_production' f b =b fold_production' g b
+    := fold_production'_extR (R := state_beq) _ _ ext b.
+  Definition fold_productions'_ext_beq
+             {f g} (ext : forall b, f b =b g b) b
+  : fold_productions' f b =b fold_productions' g b
+    := fold_productions'_extR (R := state_beq) _ _ _ ext b.
+  Definition fold_constraints_ext_beq
+             f g (H : forall x, f x =b g x) nt
+    : fold_constraints f nt =b fold_constraints g nt
+    := fold_constraints_extR (R := state_beq) _ _ _ _ _ H nt.
+
+  Global Instance fold_constraints_ProperR
+         {R : state -> state -> Prop}
+         {combine_production_Proper : Proper (R ==> R ==> R) combine_production}
+         {lub_Proper : Proper (R ==> R ==> R) least_upper_bound}
+         {R_Reflexive : Reflexive R}
+    : Proper (pointwise_relation default_nonterminal_carrierT R ==> eq ==> R)
+             fold_constraints
+  | 10.
+  Proof.
+    intros f g H; repeat intro; subst.
+    apply fold_constraints_extR; assumption.
+  Defined.
+
+  Global Instance fold_constraints_Proper
+    : Proper (pointwise_relation default_nonterminal_carrierT eq ==> eq ==> eq)
+             fold_constraints
+    := _.
+
+  Global Instance fold_constraints_Proper_state_beq
+    : Proper (pointwise_relation default_nonterminal_carrierT state_beq ==> eq ==> state_beq)
+             fold_constraints
+    := _.
+
+  Definition fixedpoint_by_abstract_interpretation : grammar_fixedpoint_data.
+  Proof.
+    refine {| prestate := T;
+              step_constraints folder nt st := fold_constraints folder nt;
+              lattice_data := fpdata |}.
+    { repeat intro; apply fold_constraints_Proper_state_beq; assumption. }
+  Defined.
 End general_fold.
 
 Section on_ensembles.
@@ -446,15 +423,12 @@ Section fold_correctness.
     }.
 
   Context {aicdata : AbstractInterpretationCorrectness}.
-  Local Hint Immediate (compile_item_data_of_abstract_interpretation G) : typeclass_instances.
-  Context (compiled_productions : list (opt.productions state))
-          (Hcompiled_productions : List.map opt.compile_productions (List.map snd (pregrammar_productions G)) = compiled_productions).
 
   Lemma fold_production_related
         (mapping : default_nonterminal_carrierT -> Ensemble String)
         st
         (Hmapping : forall nt, related (mapping nt) (st nt))
-    : forall pat, related (ensemble_fold_production' G mapping pat) (fold_production' st (opt.compile_production pat)).
+    : forall pat, related (ensemble_fold_production' G mapping pat) (fold_production' G st pat).
   Proof.
     unfold ensemble_fold_production', fold_production' in *.
     induction pat as [|[|] xs IHxs];
@@ -466,29 +440,22 @@ Section fold_correctness.
         (mapping : default_nonterminal_carrierT -> Ensemble String)
         st
         (Hmapping : forall nt, related (mapping nt) (st nt))
-    : forall pats, related (ensemble_fold_productions' G mapping pats) (fold_productions' st (opt.compile_productions pats)).
+    : forall pats, related (ensemble_fold_productions' G mapping pats) (fold_productions' G st pats).
   Proof.
     unfold ensemble_fold_productions', fold_productions' in *.
     induction pats as [|[|] xs IHxs];
       simpl;
-      repeat match goal with
-             | _ => solve [ eauto using top_related, bottom_related, lub_correct, fold_production_related ]
-             | [ |- related (ensemble_least_upper_bound _ _) _ ]
-               => apply lub_correct
-             | [ |- related (ensemble_fold_production' _ _ _) _ ]
-               => apply fold_production_related
-             end.
+      eauto using top_related, bottom_related, lub_correct, fold_production_related.
   Qed.
 
   Lemma fold_constraints_related
         (mapping : default_nonterminal_carrierT -> Ensemble String)
         st
         (Hmapping : forall nt, related (mapping nt) (st nt))
-    : forall nt, related (ensemble_fold_constraints G mapping nt) (fold_constraints compiled_productions st nt).
+    : forall nt, related (ensemble_fold_constraints G mapping nt) (fold_constraints G st nt).
   Proof.
     intro nt.
     unfold ensemble_fold_constraints, fold_constraints.
-    erewrite eq_opt_Lookup_idx by eassumption.
     apply fold_productions_related; assumption.
   Qed.
 End fold_correctness.
